---
cssclass: clean-embeds
aliases: []
tags: [_meta/literature_note, _reference/qiu_amsd]
---
# Topic[^1]
\begin{thm}  
\label{LSthm}  
Let $ E_t'(0,g,\phi)(v)$ be as in \eqref{etv}.
For $t\in F_{>0}$ and $v\in \infty$, we have
\begin{align*} &-W^{{\mathfrak{w}}}_{\infty, t}(g_\infty) \sum_{x\in K\backslash {\mathbb {V}}^{ \infty}, \ q(x)=t}\omega(g^\infty)\phi^\infty (   x) {\mathfrak{k}}(x,g_v)\\
=&
E' _t(0,g,\phi)(v) -E_t(0,g,\phi) \left(   \log \pi-(\log\Gamma)'(n+1) + \log v(t)\right). 
\end{align*}
For $t\in  F^\times$ with $v(t)<0$  for exactly   one infinite place $v$,   we have 
$$ -W^{{\mathfrak{w}}}_{\infty, t}(g_\infty)  \sum_{x\in K\backslash {\mathbb {V}}^{ \infty}, \ q(x)=t}\omega(g^\infty)\phi ^\infty(   x) {\mathfrak{k}}(x,g_v)=
E' _t(0,g,\phi)(v) .  $$
%For $t=0$, we have  $$ \omega(g)\phi (   0) {\mathfrak{k}}(0,g_\infty)=E' _0(0,g,\phi)(v) .  $$
And for $t=0$, we have $$  \omega(g)\phi (0 ) \log \delta_\infty(g_\infty)=
E' _0(0,g,\phi).  $$
\end{thm}

# See Also

# Meta
## References
![[_reference_qiu_amsd]]


## Citations and Footnotes
[^1]: Citation, thm 4.10